try SSA.v

src/SSA.v
@@ -1,58 +1,937 @@
-
-From Coq Require Import List ZArith.
+From Coq Require Import List ZArith FSets OrderedType.
 From mathcomp Require Import ssreflect ssrnat ssrbool eqtype seq ssrfun.
 From BitBlasting Require Import Typ Var TypEnv State.
-From ssrlib Require Import SsrOrdered FMaps ZAriths Tactics.
+From ssrlib Require Import SsrOrdered FMaps ZAriths Tactics Lists FSets.
 From Cryptoline Require Import DSL.
 
-(* A map from a variable to its current index *)
-Definition vmap : Type := VM.t N.
+Set Implicit Arguments.
+Unset Strict Implicit.
+Import Prenex Implicits.
 
-Definition empty_vmap : vmap := VM.empty N.
+Module M2 := Map2 VS VS.
 
-Definition initial_index : N := 0.
+Section SSA.
 
-Definition first_assigned_index : N := 1.
-
-(* Find the current index of a variable *)
-Definition get_index (v : var) (m : vmap) : N :=
-  match VM.find v m with
-  | None => initial_index
-  | Some i => i
-  end.
-
-(* Increment the current index of a variable *)
-Definition upd_index (v : var) (m : vmap) : vmap :=
-  match VM.find v m with
-  | None => VM.add v first_assigned_index m
-  | Some i => VM.add v (i + 1)%num m
-  end.
-
-Definition ssa_var (m : vmap) (v : var) : var :=
-  {| vname := vname v; vidx := get_index v m |}.
-
-Definition ssa_atomic (m : vmap) (a : atomic) : atomic :=
-  match a with
-  | Avar v => Avar (ssa_var m v)
-  | Aconst ty n => Aconst ty n
-  end.
-
-(* TODO: Define SSA translation *)
-Definition ssa_instr (m : vmap) (i : instr) : vmap * instr :=
-  match i with
-  | Imov v a =>
-    let a := ssa_atomic m a in
-    let m := upd_index v m in
-    (m, Imov (ssa_var m v) a)
-  | _ => (m, i)
-  end.
-
-(* TODO: Define SSA translation *)
-Definition ssa_program (m : vmap) (p : program) : vmap * program := (m, p).
-
-(* TODO: Define SSA translation *)
-Definition ssa_spec (s : spec) : spec := s.
+  Open Scope N_scope.
 
 
-(* TODO: Check if all variables in a program are not indexed. *)
-Definition unindexed_program (p : program) : bool := true.
+  (* A map from a variable to its current index *)
+  Definition vmap : Type := VM.t N.
+
+  Definition empty_vmap : vmap := VM.empty N.
+
+  Definition initial_index : N := 0.
+
+  Definition first_assigned_index : N := 1.
+
+  (* Find the current index of a variable *)
+  Definition get_index (v : var) (m : vmap) : N :=
+    match VM.find v m with
+    | None => initial_index
+    | Some i => i
+    end.
+
+  (* Increment the current index of a variable *)
+  Definition upd_index (v : var) (m : vmap) : vmap :=
+    match VM.find v m with
+    | None => VM.add v first_assigned_index m
+    | Some i => VM.add v (i + 1) m
+    end.
+
+  Definition ssa_var (m : vmap) (v : var) : var :=
+    {| vname := vname v; vidx := get_index v m |}.
+
+  Definition ssa_vars (m : vmap) (vs : VS.t) : VS.t :=
+    VS.Lemmas.OP.P.of_list (map (ssa_var m) (VS.elements vs)).
+
+  Definition ssa_atomic (m : vmap) (a : atomic) : atomic :=
+    match a with
+    | Avar v => Avar (ssa_var m v)
+    | Aconst ty n => Aconst ty n
+    end.
+
+  Fixpoint ssa_eexp (m: vmap) (e: eexp) :=
+    match e with
+    | Evar v => Evar (ssa_var m v)
+    | Econst c => Econst c
+    | Eunop op e => Eunop op (ssa_eexp m e)
+    | Ebinop op e1 e2 => Ebinop op (ssa_eexp m e1) (ssa_eexp m e2)
+    end.
+
+  Fixpoint ssa_rexp (m: vmap) (e: rexp) :=
+    match e with
+    | Rvar v => Rvar (ssa_var m v)
+    | Rconst w n => Rconst w n
+    | Runop w op e => Runop w op (ssa_rexp m e)
+    | Rbinop w op e1 e2 => Rbinop w op (ssa_rexp m e1) (ssa_rexp m e2)
+    | Ruext w e i => Ruext w (ssa_rexp m e) i
+    | Rsext w e i => Rsext w (ssa_rexp m e) i
+    end.
+
+  Fixpoint ssa_ebexp (m: vmap) (e: ebexp) :=
+    match e with
+    | Etrue => Etrue
+    | Eeq e1 e2 => Eeq ( ssa_eexp m e1 ) ( ssa_eexp m e2 )
+    | Eeqmod e1 e2 p => Eeqmod ( ssa_eexp m e1 ) ( ssa_eexp m e2 ) ( ssa_eexp m p )
+    | Eand e1 e2 => Eand ( ssa_ebexp m e1 ) ( ssa_ebexp m e2 )
+    end.
+
+  Fixpoint ssa_rbexp (m: vmap) (e: rbexp) :=
+    match e with
+    | Rtrue => Rtrue
+    | Req w e1 e2 => Req w ( ssa_rexp m e1 ) ( ssa_rexp m e2 )
+    | Rcmp w op e1 e2 => Rcmp w op ( ssa_rexp m e1 ) ( ssa_rexp m e2 )
+    | Rneg e => Rneg ( ssa_rbexp m e )
+    | Rand e1 e2 => Rand ( ssa_rbexp m e1 ) ( ssa_rbexp m e2 )
+    | Ror e1 e2 => Ror ( ssa_rbexp m e1 ) ( ssa_rbexp m e2 )
+    end.
+
+  Definition ssa_bexp m e := (ssa_ebexp m (eqn_bexp e) , ssa_rbexp m (rng_bexp e)).
+
+
+  Definition ssa_instr (m : vmap) (i : instr) : vmap * instr :=
+    match i with
+    | Imov v a =>
+      let a := ssa_atomic m a in
+      let m := upd_index v m in
+      (m, Imov (ssa_var m v) a)
+    | Ishl v a p =>
+      let a := ssa_atomic m a in
+      let m := upd_index v m in
+      (m, Ishl (ssa_var m v) a p)
+    | Icshl vh vl a1 a2 p =>
+      let a1 := ssa_atomic m a1 in
+      let a2 := ssa_atomic m a2 in
+      let ml := upd_index vl m in
+      let mh := upd_index vh ml in
+      (mh, Icshl (ssa_var mh vh) (ssa_var ml vl) a1 a2 p)
+    | Inondet v =>
+      let m := upd_index v m in
+      (m, Inondet (ssa_var m v))
+    | Icmov v c a1 a2 =>
+      let c := ssa_atomic m c in
+      let a1 := ssa_atomic m a1 in
+      let a2 := ssa_atomic m a2 in
+      let m := upd_index v m in
+      (m, Icmov (ssa_var m v) c a1 a2)
+    | Inop => (m, Inop)
+    | Inot v a =>
+      let a := ssa_atomic m a in
+      let m := upd_index v m in
+      (m, Inot (ssa_var m v) a)
+    | Iadd v a1 a2 =>
+      let a1 := ssa_atomic m a1 in
+      let a2 := ssa_atomic m a2 in
+      let m := upd_index v m in
+      (m, Iadd (ssa_var m v) a1 a2)
+    | Iadds c v a1 a2 =>
+      let a1 := ssa_atomic m a1 in
+      let a2 := ssa_atomic m a2 in
+      let mv := upd_index v m in
+      let mc := upd_index c mv in
+      (mc, Iadds (ssa_var mc c) (ssa_var mv v) a1 a2)
+    | Iaddr c v a1 a2 =>
+      let a1 := ssa_atomic m a1 in
+      let a2 := ssa_atomic m a2 in
+      let mv := upd_index v m in
+      let mc := upd_index c mv in
+      (mc, Iaddr (ssa_var mc c) (ssa_var mv v) a1 a2)
+    | Iadc v a1 a2 y =>
+      let a1 := ssa_atomic m a1 in
+      let a2 := ssa_atomic m a2 in
+      let y := ssa_atomic m y in
+      let m := upd_index v m in
+      (m, Iadc (ssa_var m v) a1 a2 y)
+    | Iadcs c v a1 a2 y =>
+      let a1 := ssa_atomic m a1 in
+      let a2 := ssa_atomic m a2 in
+      let y := ssa_atomic m y in
+      let mv := upd_index v m in
+      let mc := upd_index c mv in
+      (mc, Iadcs (ssa_var mc c) (ssa_var mv v) a1 a2 y)
+    | Iadcr c v a1 a2 y =>
+      let a1 := ssa_atomic m a1 in
+      let a2 := ssa_atomic m a2 in
+      let y := ssa_atomic m y in
+      let mv := upd_index v m in
+      let mc := upd_index c mv in
+      (mc, Iadcr (ssa_var mc c) (ssa_var mv v) a1 a2 y)
+    | Isub v a1 a2 =>
+      let a1 := ssa_atomic m a1 in
+      let a2 := ssa_atomic m a2 in
+      let m := upd_index v m in
+      (m, Isub (ssa_var m v) a1 a2)
+    | Isubc c v a1 a2 =>
+      let a1 := ssa_atomic m a1 in
+      let a2 := ssa_atomic m a2 in
+      let mv := upd_index v m in
+      let mc := upd_index c mv in
+      (mc, Isubc (ssa_var mc c) (ssa_var mv v) a1 a2)
+    | Isubb c v a1 a2 =>
+      let a1 := ssa_atomic m a1 in
+      let a2 := ssa_atomic m a2 in
+      let mv := upd_index v m in
+      let mc := upd_index c mv in
+      (mc, Isubb (ssa_var mc c) (ssa_var mv v) a1 a2)
+    | Isubr c v a1 a2 =>
+      let a1 := ssa_atomic m a1 in
+      let a2 := ssa_atomic m a2 in
+      let mv := upd_index v m in
+      let mc := upd_index c mv in
+      (mc, Isubr (ssa_var mc c) (ssa_var mv v) a1 a2)
+    | Isbc v a1 a2 y =>
+      let a1 := ssa_atomic m a1 in
+      let a2 := ssa_atomic m a2 in
+      let y := ssa_atomic m y in
+      let m := upd_index v m in
+      (m, Isbc (ssa_var m v) a1 a2 y)
+    | Isbcs c v a1 a2 y =>
+      let a1 := ssa_atomic m a1 in
+      let a2 := ssa_atomic m a2 in
+      let y := ssa_atomic m y in
+      let mv := upd_index v m in
+      let mc := upd_index c mv in
+      (mc, Isbcs (ssa_var mc c) (ssa_var mv v) a1 a2 y)
+    | Isbcr c v a1 a2 y =>
+      let a1 := ssa_atomic m a1 in
+      let a2 := ssa_atomic m a2 in
+      let y := ssa_atomic m y in
+      let mv := upd_index v m in
+      let mc := upd_index c mv in
+      (mc, Isbcr (ssa_var mc c) (ssa_var mv v) a1 a2 y)
+    | Isbb v a1 a2 y =>
+      let a1 := ssa_atomic m a1 in
+      let a2 := ssa_atomic m a2 in
+      let y := ssa_atomic m y in
+      let m := upd_index v m in
+      (m, Isbb (ssa_var m v) a1 a2 y)
+    | Isbbs c v a1 a2 y =>
+      let a1 := ssa_atomic m a1 in
+      let a2 := ssa_atomic m a2 in
+      let y := ssa_atomic m y in
+      let mv := upd_index v m in
+      let mc := upd_index c mv in
+      (mc, Isbbs (ssa_var mc c) (ssa_var mv v) a1 a2 y)
+    | Isbbr c v a1 a2 y =>
+      let a1 := ssa_atomic m a1 in
+      let a2 := ssa_atomic m a2 in
+      let y := ssa_atomic m y in
+      let mv := upd_index v m in
+      let mc := upd_index c mv in
+      (mc, Isbbr (ssa_var mc c) (ssa_var mv v) a1 a2 y)
+    | Imul v a1 a2 =>
+      let a1 := ssa_atomic m a1 in
+      let a2 := ssa_atomic m a2 in
+      let m := upd_index v m in
+      (m, Imul (ssa_var m v) a1 a2)
+    | Imuls c v a1 a2 =>
+      let a1 := ssa_atomic m a1 in
+      let a2 := ssa_atomic m a2 in
+      let mv := upd_index v m in
+      let mc := upd_index c mv in
+      (mc, Imuls (ssa_var mc c) (ssa_var mv v) a1 a2)
+    | Imulr c v a1 a2 =>
+      let a1 := ssa_atomic m a1 in
+      let a2 := ssa_atomic m a2 in
+      let mv := upd_index v m in
+      let mc := upd_index c mv in
+      (mc, Imulr (ssa_var mc c) (ssa_var mv v) a1 a2)
+    | Imull vh vl a1 a2 =>
+      let a1 := ssa_atomic m a1 in
+      let a2 := ssa_atomic m a2 in
+      let ml := upd_index vl m in
+      let mh := upd_index vh ml in
+      (mh, Imull (ssa_var mh vh) (ssa_var ml vl) a1 a2)
+    | Imulj v a1 a2 =>
+      let a1 := ssa_atomic m a1 in
+      let a2 := ssa_atomic m a2 in
+      let m := upd_index v m in
+      (m, Imulj (ssa_var m v) a1 a2)
+    | Isplit vh vl a n =>
+      let a := ssa_atomic m a in
+      let ml := upd_index vl m in
+      let mh := upd_index vh ml in
+      (mh, Isplit (ssa_var mh vh) (ssa_var ml vl) a n)
+    | Iand v a1 a2 =>
+      let a1 := ssa_atomic m a1 in
+      let a2 := ssa_atomic m a2 in
+      let m := upd_index v m in
+      (m, Iand (ssa_var m v) a1 a2)
+    | Ior v a1 a2 =>
+      let a1 := ssa_atomic m a1 in
+      let a2 := ssa_atomic m a2 in
+      let m := upd_index v m in
+      (m, Ior (ssa_var m v) a1 a2)
+    | Ixor v a1 a2 =>
+      let a1 := ssa_atomic m a1 in
+      let a2 := ssa_atomic m a2 in
+      let m := upd_index v m in
+      (m, Ixor (ssa_var m v) a1 a2)
+    | Icast v a =>
+      let a := ssa_atomic m a in
+      let m := upd_index v m in
+      (m, Imov (ssa_var m v) a)
+    | Ivpc v a =>
+      let a := ssa_atomic m a in
+      let m := upd_index v m in
+      (m, Imov (ssa_var m v) a)
+    | Ijoin v ah al =>
+      let ah := ssa_atomic m ah in
+      let al := ssa_atomic m al in
+      let m := upd_index v m in
+      (m, Ijoin (ssa_var m v) ah al)
+    | Iassert e => (m, Iassert (ssa_bexp m e))
+    | Iassume e => (m, Iassume (ssa_bexp m e))
+    | Iecut e pwss => (m, Iecut ( ssa_ebexp m e ) pwss)
+    | Ircut e pwss => (m, Ircut ( ssa_rbexp m e ) pwss)
+    | Ighost vs e => (m, Ighost (ssa_vars m vs) (ssa_bexp m e))
+                      (* | _ => (m, i) *)
+    end.
+
+  Fixpoint ssa_program (m : vmap) (p : program) : vmap * program :=
+    match p with
+    | [::] => (m, [::])
+    | hd::tl =>
+      let (m, hd) := ssa_instr m hd in
+      let (m, tl) := ssa_program m tl in
+      (m, hd::tl)
+    end.
+
+  (* TODO: Define SSA translation *)
+  Definition ssa_spec (s : spec) : spec :=
+    let m := empty_vmap in
+    let f := ssa_bexp m (spre s) in
+    let (m, p) := ssa_program m (sprog s) in
+    let g := ssa_bexp m (spost s) in
+    {| sinputs := (sinputs s);
+       spre := f;
+       sprog := p;
+       spost := g;
+       sepwss := (sepwss s);
+       srpwss := (srpwss s);
+    |}.
+
+
+  (* TODO: Check if all variables in a program are not indexed. *)
+
+  Definition unindexed_var (v : var) : bool :=
+    vidx v == 0.
+
+  Definition unindexed_vars vs := VS.for_all unindexed_var vs.
+
+  Definition unindexed_atomic  (a : atomic) : bool :=
+    match a with
+    | Avar v => unindexed_var v
+    | Aconst ty n => true
+    end.
+
+  Fixpoint unindexed_eexp (e: eexp) :=
+    match e with
+    | Evar v => unindexed_var v
+    | Econst c => true
+    | Eunop op e => unindexed_eexp e
+    | Ebinop op e1 e2 => unindexed_eexp e1 && unindexed_eexp e2
+    end.
+
+  Fixpoint unindexed_rexp (e: rexp) :=
+    match e with
+    | Rvar v => unindexed_var v
+    | Rconst w n => true
+    | Runop w op e => unindexed_rexp e
+    | Rbinop w op e1 e2 => unindexed_rexp e1 && unindexed_rexp e2
+    | Ruext w e i => unindexed_rexp e
+    | Rsext w e i => unindexed_rexp e
+    end.
+
+  Fixpoint unindexed_ebexp (e: ebexp) :=
+    match e with
+    | Etrue => true
+    | Eeq e1 e2 => unindexed_eexp e1 && unindexed_eexp e2
+    | Eeqmod e1 e2 p => unindexed_eexp e1 && unindexed_eexp e2 && unindexed_eexp p
+    | Eand e1 e2 => unindexed_ebexp e1 && unindexed_ebexp e2
+    end.
+
+  Fixpoint unindexed_rbexp (e: rbexp) :=
+    match e with
+    | Rtrue => true
+    | Req w e1 e2 => unindexed_rexp e1 && unindexed_rexp e2
+    | Rcmp w op e1 e2 => unindexed_rexp e1 && unindexed_rexp e2
+    | Rneg e =>  unindexed_rbexp e
+    | Rand e1 e2 => unindexed_rbexp e1 && unindexed_rbexp e2
+    | Ror e1 e2 => unindexed_rbexp e1 && unindexed_rbexp e2
+    end.
+
+  Definition unindexed_bexp e := unindexed_ebexp (eqn_bexp e) && unindexed_rbexp (rng_bexp e).
+
+  Definition unindexed_instr (i: instr) : bool :=
+    match i with
+    | Imov v a
+    | Ishl v a _ =>
+      let v := unindexed_var v in
+      let a := unindexed_atomic a in
+      v && a
+    | Icshl vh vl a1 a2 _ =>
+      let vh := unindexed_var vh in
+      let vl := unindexed_var vl in
+      let a1 := unindexed_atomic a1 in
+      let a2 := unindexed_atomic a2 in
+      vh && vl && a1 && a2
+    | Inondet v =>
+      let v := unindexed_var v in v
+    | Icmov v c a1 a2 =>
+      let v := unindexed_var v in
+      let c := unindexed_atomic c in
+      let a1 := unindexed_atomic a1 in
+      let a2 := unindexed_atomic a2 in
+      v && c && a1 && a2
+    | Inop => true
+    | Inot v a =>
+      let v := unindexed_var v in
+      let a := unindexed_atomic a in
+      v && a
+    | Iadd v a1 a2 =>
+      let v := unindexed_var v in
+      let a1 := unindexed_atomic a1 in
+      let a2 := unindexed_atomic a2 in
+      v && a1 && a2
+    | Iadds c v a1 a2
+    | Iaddr c v a1 a2 =>
+      let c := unindexed_var c in
+      let v := unindexed_var v in
+      let a1 := unindexed_atomic a1 in
+      let a2 := unindexed_atomic a2 in
+      c && v && a1 && a2
+    | Iadc v a1 a2 y =>
+      let v := unindexed_var v in
+      let a1 := unindexed_atomic a1 in
+      let a2 := unindexed_atomic a2 in
+      let y := unindexed_atomic y in
+      v && a1 && a2 && y
+    | Iadcs c v a1 a2 y
+    | Iadcr c v a1 a2 y =>
+      let c := unindexed_var c in
+      let v := unindexed_var v in
+      let a1 := unindexed_atomic a1 in
+      let a2 := unindexed_atomic a2 in
+      let y := unindexed_atomic y in
+      c && v && a1 && a2 && y
+    | Isub v a1 a2 =>
+      let v := unindexed_var v in
+      let a1 := unindexed_atomic a1 in
+      let a2 := unindexed_atomic a2 in
+      v && a1 && a2
+    | Isubc c v a1 a2
+    | Isubb c v a1 a2
+    | Isubr c v a1 a2 =>
+      let c := unindexed_var c in
+      let v := unindexed_var v in
+      let a1 := unindexed_atomic a1 in
+      let a2 := unindexed_atomic a2 in
+      c && v && a1 && a2
+    | Isbc v a1 a2 y =>
+      let v := unindexed_var v in
+      let a1 := unindexed_atomic a1 in
+      let a2 := unindexed_atomic a2 in
+      let y := unindexed_atomic y in
+      v && a1 && a2 && y
+    | Isbcs c v a1 a2 y
+    | Isbcr c v a1 a2 y =>
+      let c := unindexed_var c in
+      let v := unindexed_var v in
+      let a1 := unindexed_atomic a1 in
+      let a2 := unindexed_atomic a2 in
+      let y := unindexed_atomic y in
+      c && v && a1 && a2 && y
+    | Isbb v a1 a2 y =>
+      let v := unindexed_var v in
+      let a1 := unindexed_atomic a1 in
+      let a2 := unindexed_atomic a2 in
+      let y := unindexed_atomic y in
+      v && a1 && a2 && y
+    | Isbbs c v a1 a2 y
+    | Isbbr c v a1 a2 y =>
+      let c := unindexed_var c in
+      let v := unindexed_var v in
+      let a1 := unindexed_atomic a1 in
+      let a2 := unindexed_atomic a2 in
+      let y := unindexed_atomic y in
+      c && v && a1 && a2 && y
+    | Imul v a1 a2 =>
+      let v := unindexed_var v in
+      let a1 := unindexed_atomic a1 in
+      let a2 := unindexed_atomic a2 in
+      v && a1 && a2
+    | Imuls c v a1 a2
+    | Imulr c v a1 a2 =>
+      let c := unindexed_var c in
+      let v := unindexed_var v in
+      let a1 := unindexed_atomic a1 in
+      let a2 := unindexed_atomic a2 in
+      c && v && a1 && a2
+    | Imull vh vl a1 a2 =>
+      let vh := unindexed_var vh in
+      let vl := unindexed_var vl in
+      let a1 := unindexed_atomic a1 in
+      let a2 := unindexed_atomic a2 in
+      vh && vl && a1 && a2
+    | Imulj v a1 a2 =>
+      let v := unindexed_var v in
+      let a1 := unindexed_atomic a1 in
+      let a2 := unindexed_atomic a2 in
+      v && a1 && a2
+    | Isplit vh vl a n =>
+      let vh := unindexed_var vh in
+      let vl := unindexed_var vl in
+      let a := unindexed_atomic a in
+      vh && vl && a
+    | Iand v a1 a2
+    | Ior v a1 a2
+    | Ixor v a1 a2 =>
+      let v := unindexed_var v in
+      let a1 := unindexed_atomic a1 in
+      let a2 := unindexed_atomic a2 in
+      v && a1 && a2
+    | Icast v a
+    | Ivpc v a =>
+      let v := unindexed_var v in
+      let a := unindexed_atomic a in
+      v && a
+    | Ijoin v ah al =>
+      let v := unindexed_var v in
+      let ah := unindexed_atomic ah in
+      let al := unindexed_atomic al in
+      v && ah && al
+    | Iassert e => unindexed_bexp e
+    | Iassume e => unindexed_bexp e
+    | Iecut e pwss => unindexed_ebexp e
+    | Ircut e pwss => unindexed_rbexp e
+    | Ighost vs e => unindexed_vars vs && unindexed_bexp e
+    end.
+
+  Fixpoint unindexed_program (p : program) : bool :=
+    match p with
+    | [::] => true
+    | hd::tl =>
+      let unidx_instr := unindexed_instr hd in
+      let unidx_tl := unindexed_program tl in
+      unidx_instr && unidx_tl
+    end.
+
+  Lemma ssa_program_empty : forall m, ssa_program m [::] = (m, [::]).
+  Proof.
+    reflexivity.
+  Qed.
+
+  Lemma ssa_program_cons :
+    forall m1 m2 hd tl p,
+      ssa_program m1 (hd::tl) = (m2, p) ->
+      exists m3 h t,
+        ssa_instr m1 hd = (m3, h) /\ ssa_program m3 tl = (m2, t) /\ p = h::t.
+  Proof.
+    move=> m1 m2 hd tl p /=.
+    set tmp := ssa_instr m1 hd.
+    have: (tmp = ssa_instr m1 hd) by reflexivity.
+    destruct tmp as [m3 h].
+    set tmp := ssa_program m3 tl.
+    have: (tmp = ssa_program m3 tl) by reflexivity.
+    destruct tmp as [m4 t].
+    move=> Htl Hhd [] Hm Hp.
+    exists m3; exists h; exists t; split; [idtac | split].
+    - reflexivity.
+    - rewrite -Htl Hm.
+      reflexivity.
+    - symmetry; exact: Hp.
+  Qed.
+
+  Lemma ssa_spec_unfold s :
+    exists m, spre (ssa_spec s) = ssa_bexp empty_vmap (spre s) /\
+         (m, sprog (ssa_spec s)) = ssa_program empty_vmap (sprog s) /\
+         spost (ssa_spec s) = ssa_bexp m (spost s).
+  Proof.
+    destruct s as [f p g] => /=.
+    rewrite /ssa_spec /=.
+    set tmp := ssa_program empty_vmap g.
+    destruct tmp as [m sp] => /=.
+    exists m; split; [idtac | split]; reflexivity.
+  Qed.
+
+  Lemma get_index_empty v :
+    get_index v empty_vmap = 0.
+  Proof.
+    done.
+  Qed.
+
+  Lemma get_index_add_eq x y i s :
+    x == y ->
+    get_index x (VM.add y i s) = i.
+  Proof.
+    move=> Heq.
+    rewrite (eqP Heq) /get_index (VM.Lemmas.add_eq_o _ _ (eqxx y)).
+    reflexivity.
+  Qed.
+
+  Lemma get_index_add_neq x y i s :
+    x != y ->
+    get_index x (VM.add y i s) = get_index x s.
+  Proof.
+    move=> /negP Hne.
+    rewrite eq_sym in Hne.
+    rewrite /get_index (VM.Lemmas.add_neq_o _ _ Hne).
+    reflexivity.
+  Qed.
+
+  Lemma get_upd_index_gt0 :
+    forall (m : vmap) (v : var),
+      0 <? get_index v (upd_index v m).
+  Proof.
+    move=> m v; rewrite /upd_index.
+    case: (VM.find v m) => /=.
+    - move=> a.
+      rewrite (get_index_add_eq _ _ (eqxx v)).
+      exact: Nltn0Sn.
+    - rewrite (get_index_add_eq _ _ (eqxx v)).
+      done.
+  Qed.
+
+  Lemma get_upd_index_lt :
+    forall (m : vmap) (v : var),
+      get_index v m <? get_index v (upd_index v m).
+  Proof.
+    move=> m v; rewrite /upd_index /get_index.
+    case: (VM.find v m) => /=.
+    - move=> a.
+      rewrite (VM.Lemmas.add_eq_o _ _ (eqxx v)).
+      exact: NltnSn.
+    - rewrite (VM.Lemmas.add_eq_o _ _ (eqxx v)).
+      done.
+  Qed.
+
+  Lemma get_upd_index_leF :
+    forall (m : vmap) (v : var),
+      get_index v (upd_index v m) <=? get_index v m -> False.
+  Proof.
+    move=> m v Hle.
+    move: (get_upd_index_lt m v) => Hlt.
+    move: (Nleq_ltn_trans Hle Hlt).
+    rewrite Nltnn.
+    done.
+  Qed.
+
+  Lemma get_upd_index_eq :
+    forall (m : vmap) (v : var),
+      get_index v (upd_index v m) = get_index v m + 1.
+  Proof.
+    move=> m v.
+    rewrite /upd_index.
+    case H: (VM.find v m).
+    - rewrite /get_index.
+      rewrite (VM.Lemmas.add_eq_o m _ (eqxx v)).
+      rewrite H.
+      reflexivity.
+    - rewrite /get_index.
+      rewrite (VM.Lemmas.add_eq_o m _ (eqxx v)).
+      rewrite H.
+      reflexivity.
+  Qed.
+
+  Lemma get_upd_index_neq :
+    forall (m : vmap) (x v : var),
+      x != v ->
+      get_index x (upd_index v m) = get_index x m.
+  Proof.
+    move=> m x v => /negP Hne.
+    rewrite eq_sym in Hne.
+    rewrite /upd_index /get_index.
+    case: (VM.find v m).
+    - move=> a.
+      rewrite (VM.Lemmas.add_neq_o _ _ Hne).
+      reflexivity.
+    - rewrite (VM.Lemmas.add_neq_o _ _ Hne).
+      reflexivity.
+  Qed.
+
+  Lemma get_upd_index_le :
+    forall (m : vmap) (x v : var),
+      get_index x m <=? get_index x (upd_index v m).
+  Proof.
+    move=> m x v.
+    case Hxv: (x == v).
+    - move: (get_upd_index_lt m v) => Hlt.
+      rewrite (eqP Hxv).
+      exact: (NltnW Hlt).
+    - move/idP/negP: Hxv => Hxv.
+      rewrite (get_upd_index_neq _ Hxv).
+      exact: Nleqnn.
+  Qed.
+
+  Lemma ssa_instr_index_le :
+    forall m1 m2 v i si,
+      ssa_instr m1 i = (m2, si) ->
+      get_index v m1 <=? get_index v m2.
+  Proof.
+    move=> m1 m2 v i si.
+    elim: i m1 m2 v si; intros;
+      (let rec tac :=
+           match goal with
+           | H: ssa_instr _ _ = (_, _) |- _ =>
+             case: H => <- Hsi; tac
+           | |- is_true (get_index ?v ?m1 <=? get_index ?v (upd_index ?t ?m1)) =>
+             exact: get_upd_index_le
+           | |- is_true (get_index ?v ?m1 <=? get_index ?v (upd_index ?vl (upd_index ?vh m1))) =>
+             move: (get_upd_index_le m1 v vh) => Hle1; move: (get_upd_index_le (upd_index vh m1) v vl) => Hle2; exact: (Nleq_trans Hle1 Hle2)
+           | |- is_true (get_index ?v ?m <=? get_index ?v ?m) => exact: Nleqnn
+           | |- _ => idtac
+           end in
+       tac).
+  Qed.
+
+  Lemma ssa_program_index_le :
+    forall m1 m2 v p sp,
+      ssa_program m1 p = (m2, sp) ->
+      get_index v m1 <=? get_index v m2.
+  Proof.
+    move=> m1 m2 v p sp.
+    elim: p m1 m2 v sp.
+    - move=> m1 m2 v sp Hsp.
+      rewrite ssa_program_empty in Hsp.
+      case: Hsp => Hm1 Hsp.
+      rewrite Hm1; exact: Nleqnn.
+    - move=> hd tl IH m1 m2 v sp Hsp.
+      move: (ssa_program_cons Hsp) => {Hsp} [m3 [shd [stl [Hshd [Hstl Hsp]]]]].
+      move: (ssa_instr_index_le v Hshd) => Hle1.
+      move: (IH _ _ v _ Hstl) => Hle2.
+      exact: (Nleq_trans Hle1 Hle2).
+  Qed.
+
+
+  Lemma ssa_var_upd_eq v m :
+    ssa_var (upd_index v m) v = {|vname := vname v; vidx := get_index v (upd_index v m) |}.
+  Proof.
+    reflexivity.
+  Qed.
+
+  Lemma ssa_var_upd_neq x v m :
+    x != v ->
+    ssa_var (upd_index v m) x = ssa_var m x.
+  Proof.
+    move=> Hxv.
+    rewrite /ssa_var.
+    rewrite (get_upd_index_neq _ Hxv).
+    reflexivity.
+  Qed.
+
+  Lemma ssa_vars_mem_elements m v vs :
+    VS.mem v (ssa_vars m vs) = (v \in (VS.elements (ssa_vars m vs))).
+  Proof.
+    move: (VS.Lemmas.elements_iff (ssa_vars m vs) v) => [HinA Hin].
+    case Hv: (v \in VS.elements (ssa_vars m vs)).
+    - move/InAP: Hv => Hv.
+      apply/VS.Lemmas.memP.
+      apply: Hin.
+      assumption.
+    - move/negP: Hv => Hv.
+      apply/negP => /VS.Lemmas.memP Hmem.
+      apply: Hv.
+      apply/InAP.
+      apply: HinA.
+      assumption.
+  Qed.
+
+  Lemma ssa_vars_Empty m vs :
+    VS.Empty vs ->
+    VS.Empty (ssa_vars m vs).
+  Proof.
+    rewrite /ssa_vars.
+    move=> Hempty.
+    apply VS.Lemmas.OP.P.elements_Empty in Hempty.
+    rewrite /M2.map2.
+    rewrite Hempty.
+    rewrite /=.
+    exact: VS.empty_1.
+  Qed.
+
+  Lemma ssa_var_preserve m x y : x == y -> ssa_var m x == ssa_var m y.
+  Proof.
+    move=> H.
+    rewrite (eqP H).
+    exact: eqxx.
+  Qed.
+
+  Lemma ssa_var_injective m x y :
+    unindexed_var x ->
+    unindexed_var y ->
+    ssa_var m x == ssa_var m y ->
+    x == y.
+  Proof.
+    rewrite /unindexed_var.
+    move=> Hu1 Hu2 /eqP H.
+    case: H => H H2.
+    have: (x =? y)%var by rewrite /var_eqn H (eqP Hu1) (eqP Hu2) !eqxx.
+      by move/var_eqP -> .
+  Qed.
+
+  Lemma inA_ssa_var_map1 m x s :
+    InA VS.E.eq x s ->
+    InA VS.E.eq (ssa_var m x) (map (ssa_var m) s).
+  Proof.
+    elim: s m x => /=.
+    - move=> m x H; by inversion H.
+    - move=> hd tl IH m x Hin.
+      inversion_clear Hin.
+      + apply: InA_cons_hd.
+        exact: (ssa_var_preserve m H).
+      + apply: InA_cons_tl.
+        exact: (IH _ _ H).
+  Qed.
+
+  Lemma inA_ssa_var_map2 m x s :
+    unindexed_var x ->
+    all unindexed_var s ->
+    InA VS.E.eq (ssa_var m x) (map (ssa_var m) s) ->
+    InA VS.E.eq x s.
+  Proof.
+    elim: s m x => /=.
+    - move=> m x Hu _ H; by inversion H.
+    - move=> hd tl IH m x Hux /andP [Huhd Hutl] Hin.
+      inversion_clear Hin.
+      + apply: InA_cons_hd.
+        exact: (ssa_var_injective Hux Huhd H).
+      + apply: InA_cons_tl.
+        exact: (IH _ _ _ _ H).
+  Qed.
+
+  Lemma inA_ssa_var_map3 m x s :
+    InA VS.E.eq x (map (ssa_var m) s) ->
+    exists y, VS.E.eq x (ssa_var m y) /\ InA VS.E.eq y s.
+  Proof.
+    elim: s m x => /=.
+    - move=> x m H; by inversion H.
+    - move=> hd tl IH x m Hin.
+      inversion_clear Hin.
+      + exists hd; split.
+        * assumption.
+        * apply: InA_cons_hd.
+          exact: VS.E.eq_refl.
+      + move: (IH _ _ H) => [y [Heq HinA]].
+        exists y; split.
+        * assumption.
+        * exact: InA_cons_tl.
+  Qed.
+
+  Definition ssa_var_map2 m s :=
+    VS.Lemmas.OP.P.of_list (map (ssa_var m) (VS.elements s)).
+
+  Lemma map2_Empty1 m s :
+    VS.Empty s ->
+    VS.Empty (ssa_var_map2 m s).
+  Proof.
+    move=> Hemp1.
+    rewrite /ssa_var_map2.
+    move=> x Hin.
+    move: (VS.Lemmas.OP.P.elements_Empty s) => [H _].
+    rewrite (H Hemp1) /= in Hin => {H}.
+    move: (VS.Lemmas.empty_iff x) => [H _].
+    apply: H; assumption.
+  Qed.
+
+  Lemma ssa_var_map2_Empty2 m s :
+    VS.Empty (ssa_var_map2 m s) ->
+    VS.Empty s.
+  Proof.
+    move=> Hemp1.
+    rewrite /ssa_var_map2 in Hemp1.
+    move=> x Hmem.
+    apply: (Hemp1 (ssa_var m x)).
+    apply: VS.Lemmas.in_of_list2.
+    apply: inA_ssa_var_map1.
+    exact: (VS.elements_1 Hmem).
+  Qed.
+
+  Lemma compat_unindexed_var: compat_bool VS.TS.SE.eq unindexed_var.
+  Proof.
+    rewrite /compat_bool /Proper.
+    rewrite /respectful /impl.
+    move=> a b H1.
+    inversion H1.
+      by rewrite (eqP H0).
+  Qed.
+
+  Lemma ssa_var_map2_mem1 m (x: var) xs :
+    unindexed_var x ->
+    unindexed_vars xs ->
+    VS.mem (ssa_var m x) (ssa_vars m xs) = VS.mem x xs.
+  Proof.
+    move=> Hux Huxs.
+    case Hmem1: (VS.mem x xs).
+    - apply: VS.Lemmas.mem_of_list2.
+      apply: inA_ssa_var_map1.
+      move/VS.Lemmas.memP: Hmem1 => Hin1.
+      exact: (VS.elements_1 Hin1).
+    - apply/negP => Hmem2.
+      move/negP: Hmem1; apply.
+      move: (VS.Lemmas.mem_of_list1 Hmem2) => HinA.
+      rewrite /unindexed_vars in Huxs.
+      move: (VS.Lemmas.for_all_b xs compat_unindexed_var) => H2.
+      rewrite H2 in Huxs.
+      move: (inA_ssa_var_map2 Hux Huxs HinA) => {HinA} HinA.
+      apply/VS.Lemmas.memP.
+      exact: (VS.elements_2 HinA).
+  Qed.
+
+  Lemma ssa_var_map2_mem2 m x xs :
+    VS.mem x (ssa_var_map2 m xs) ->
+    exists y, VS.E.eq x (ssa_var m y) /\ VS.mem y xs.
+  Proof.
+    rewrite /ssa_var_map2 => Hmem.
+    move: (VS.Lemmas.mem_of_list1 Hmem) => {Hmem} HinA.
+    move: (inA_ssa_var_map3 HinA) => {HinA} [y [Heq HinA]].
+    exists y; split.
+    - assumption.
+    - apply/VS.Lemmas.memP.
+      exact: VS.elements_2.
+  Qed.
+
+  Lemma ssa_var_map2_singleton m x :
+    unindexed_var x ->
+    unindexed_vars (VS.singleton x) ->
+    VS.Equal (ssa_var_map2 m (VS.singleton x)) (VS.singleton (ssa_var m x)).
+  Proof.
+    move=> Hux Huxs v; split => /VS.Lemmas.memP Hmem; apply: VS.Lemmas.memP.
+    - move: (ssa_var_map2_mem2 Hmem) => [y [Hy Hmemy]].
+      apply: VS.Lemmas.mem_singleton2. rewrite (eqP Hy).
+      exact: (ssa_var_preserve m (VS.Lemmas.mem_singleton1 Hmemy)).
+    - rewrite (eqP (VS.Lemmas.mem_singleton1 Hmem)) (ssa_var_map2_mem1 m Hux Huxs).
+      apply: VS.Lemmas.mem_singleton2. exact: VS.E.eq_refl.
+  Qed.
+
+  Lemma ssa_vars_mem1 m v vs :
+    unindexed_var v ->
+    unindexed_vars vs ->
+    VS.mem (ssa_var m v) (ssa_vars m vs) = VS.mem v vs.
+  Proof.
+    move=> Hux Huxs.
+    exact: (ssa_var_map2_mem1 m Hux Huxs).
+  Qed.
+
+  Lemma ssa_vars_mem2 m v vs :
+    VS.mem v (ssa_vars m vs) ->
+    exists x, v = ssa_var m x /\ VS.mem x vs.
+  Proof.
+    move=> Hmem; move: (ssa_var_map2_mem2 Hmem) => [y [/eqP Hy Hmemy]].
+    rewrite Hy.
+      by exists y.
+  Qed.
+
+  Lemma ssa_vars_mem3 m v i vs :
+    unindexed_var v ->
+    unindexed_vars vs ->
+    VS.mem v vs ->
+    i = get_index v m ->
+    VS.mem {| vname := vname v; vidx :=i |} (ssa_vars m vs).
+  Proof.
+    move=> Hux Huxs Hmem Hidx.
+    rewrite Hidx.
+    rewrite (ssa_vars_mem1 m Hux Huxs).
+    assumption.
+  Qed.
+End SSA.
